Setlec/Verify/PairM.lean
@@ -129,11 +129,11 @@ theorem iotaCerts_fst (d : Nat) :
   | _, [] => rfl
   | .forallE n ty body mb, arg :: rest => by
     show ((do
-        let ta ← (pairFns r₁ r₂ h).infer d arg
+        let ta ← (pairFns r₁ r₂ h).inferIO d arg
         if ← (pairFns r₁ r₂ h).defeq d ta ty then
           iotaCerts (pairFns r₁ r₂ h) env d (body.instantiate1 arg) rest
         else pure false : PairM rel Bool)).val.1 = (do
-        let ta ← r₁.infer d arg
+        let ta ← r₁.inferIO d arg
         if ← r₁.defeq d ta ty then
           iotaCerts r₁ env d (body.instantiate1 arg) rest
         else pure false)
@@ -159,11 +159,11 @@ theorem iotaCerts_snd (d : Nat) :
   | _, [] => rfl
   | .forallE n ty body mb, arg :: rest => by
     show ((do
-        let ta ← (pairFns r₁ r₂ h).infer d arg
+        let ta ← (pairFns r₁ r₂ h).inferIO d arg
         if ← (pairFns r₁ r₂ h).defeq d ta ty then
           iotaCerts (pairFns r₁ r₂ h) env d (body.instantiate1 arg) rest
         else pure false : PairM rel Bool)).val.2 = (do
-        let ta ← r₂.infer d arg
+        let ta ← r₂.inferIO d arg
         if ← r₂.defeq d ta ty then
           iotaCerts r₂ env d (body.instantiate1 arg) rest
         else pure false)
